RocqOfRust/revm/revm_interpreter/gas/links/calc.v
@@ -161,20 +161,6 @@ Proof.
 Defined.
 Global Opaque run_static_sstore_cost.
 
-(* pub const fn dyn_sstore_cost(spec_id: SpecId, vals: &SStoreResult, is_cold: bool) -> u64 *)
-Instance run_dyn_sstore_cost
-    (spec_id : SpecId.t)
-    (vals : '& SStoreResult.t)
-    (is_cold : bool) :
-  Run.Trait
-    gas.calc.dyn_sstore_cost [] [] [ φ spec_id; φ vals; φ is_cold ]
-    u64.
-Proof.
-  constructor.
-  run_symbolic.
-Admitted.
-Global Opaque run_dyn_sstore_cost.
-
 (* pub fn sstore_cost(spec_id: SpecId, vals: &SStoreResult, is_cold: bool) -> u64 *)
 Instance run_sstore_cost
     (spec_id : SpecId.t)
@@ -188,6 +174,24 @@ Proof.
   run_symbolic.
 Admitted.
 Global Opaque run_sstore_cost.
+
+(* pub const fn dyn_sstore_cost(spec_id: SpecId, vals: &SStoreResult, is_cold: bool) -> u64 *)
+Instance run_dyn_sstore_cost
+    (spec_id : SpecId.t)
+    (vals : '& SStoreResult.t)
+    (is_cold : bool) :
+  Run.Trait
+    gas.calc.dyn_sstore_cost [] [] [ φ spec_id; φ vals; φ is_cold ]
+    u64.
+Proof.
+  constructor.
+  run_symbolic.
+  Unshelve.
+  all: try eapply run_sstore_cost.
+  all: try eapply run_static_sstore_cost.
+  all: try typeclasses eauto.
+Defined.
+Global Opaque run_dyn_sstore_cost.
 
 (* pub const fn istanbul_sstore_cost<const SLOAD_GAS: u64, const SSTORE_RESET_GAS: u64>(
     vals: &SStoreResult,
